theories/case_studies/multiuser_kvs/kvs_spec_search.v
@@ -17,17 +17,17 @@ Section KVS_search.
   Lemma KVS_search_spec_in `{KVS : kvsLayout}
     (pc_b pc_e pc_a : Addr)
     (cgp_b cgp_e : Addr)
-    (rkey ridx rscratch : RegName)
+    (rkey ridx ridx_empty rscratch : RegName)
     (m : kvs_map) (s : kvs_alloc) (idx : nat) (fkey : Z) (w : Word)
     :
-    let instrs := (kvs_search_instrs rkey ridx rscratch) in
+    let instrs := (kvs_search_instrs rkey ridx ridx_empty rscratch) in
     SubBounds pc_b pc_e pc_a (pc_a ^+ length instrs)%a ->
     withinBounds cgp_b cgp_e cgp_b = true ->
-    ((cgp_b + (2*SIZE_MAP)%Z)%a = Some cgp_e)%a ->
-    fkey ≠ EMPTY_SLOT ->
+    ((cgp_b + (3*SIZE_MAP)%Z)%a = Some cgp_e)%a ->
 
     rscratch ≠ cnull ->
     ridx ≠ cnull ->
+    ridx_empty ≠ cnull ->
     rkey ≠ cnull ->
 
     (
@@ -35,6 +35,7 @@ Section KVS_search.
       cgp ↦ᵣ WCap RW Global cgp_b cgp_e cgp_b ∗
       rkey ↦ᵣ WInt fkey ∗
       ridx ↦ᵣ - ∗
+      ridx_empty ↦ᵣ - ∗
       rscratch ↦ᵣ - ∗
 
       isKVS cgp_b m s ∗
@@ -43,19 +44,20 @@ Section KVS_search.
       codefrag pc_a instrs ∗
       ▷ (
           PC ↦ᵣ WCap RX Global pc_b pc_e (pc_a ^+ length instrs)%a ∗
-          cgp ↦ᵣ WCap RW Global cgp_b cgp_e (cgp_b ^+ (2*idx) )%a ∗
+          cgp ↦ᵣ WCap RW Global cgp_b cgp_e (cgp_b ^+ (3*idx) )%a ∗
           rkey ↦ᵣ WInt fkey ∗
           ridx ↦ᵣ WInt idx ∗
+          ridx_empty ↦ᵣ - ∗
           rscratch ↦ᵣ - ∗
 
           isKVS_open cgp_b m s idx ∗
-          (cgp_b ^+ (2*idx))%a ↦ₐ WInt fkey ∗
-          (cgp_b ^+ (2*idx + 1))%a ↦ₐ w ∗
-          isKVS_entry_empty idx fkey ∗
-
-          ⌜ withinBounds cgp_b cgp_e (cgp_b ^+ (2 * idx + 1))%a = true ⌝ ∗
-
+          (cgp_b ^+ (3*idx))%a ↦ₐ WInt ASM_SOME ∗
+          (cgp_b ^+ (3*idx + 1))%a ↦ₐ WInt fkey ∗
+          (cgp_b ^+ (3*idx + 2))%a ↦ₐ w ∗
           fkey ⤇(KVS)[idx] w ∗
+
+          ⌜ withinBounds cgp_b cgp_e (cgp_b ^+ (3 * idx + 2))%a = true ⌝ ∗
+
           codefrag pc_a instrs -∗
 
           WP Seq (Instr Executable) {{ v, ⌜v = HaltedV⌝ → na_own cerise_nais ⊤ }}
@@ -63,22 +65,28 @@ Section KVS_search.
       ⊢ WP Seq (Instr Executable) {{ v, ⌜v = HaltedV⌝ → na_own cerise_nais ⊤ }})%I.
   Proof.
     intros instrs ; subst instrs.
-    iIntros (HsubBounds Hbounds_cgp Hcgp_bound Hfkey_ne_empty Hrscratch Hridx Hkey)
-      "(HPC & Hcgp & Hrkey & [%widx Hridx] & Hrscratch & HKVS & Hkvs_frag & Hcode & Hpost)".
+    iIntros (HsubBounds Hbounds_cgp Hcgp_bound Hrscratch Hridx Hridx_empty Hkey)
+      "(HPC & Hcgp & Hrkey & [%widx Hridx] & [%widx_empty Hridx_empty] & Hrscratch
+      & HKVS & Hkvs_frag & Hcode & Hpost)".
     codefrag_facts "Hcode"; rename H into Hpc_contiguous ; clear H0.
 
-    (* Mov ridx 0 *)
+
+    (* mov ridx 0%Z; *)
+    iInstr "Hcode".
+    (* mov ridx_empty (-1)%Z; *)
     iInstr "Hcode".
 
     remember 0%Z as n.
     iAssert (⌜ (0 <= n <= SIZE_MAP)%Z ⌝)%I as "%Hn"; first (iPureIntro ; lia).
-    rewrite{2} (_ : (cgp_b = (cgp_b ^+ (2 * n))%a)); last by solve_addr.
-    assert (forall i, (0 <= i < Z.to_nat n) -> ∃ (k : Z) (w : Word),  m !! i = Some (k,w) ∧ k ≠ fkey)
+    rewrite{2} (_ : (cgp_b = (cgp_b ^+ (3 * n))%a)); last by solve_addr.
+    assert (forall i, (0 <= i < Z.to_nat n) -> ∀ (k : Z) (w : Word),
+                m !! i = Some (Some (k,w)) -> k ≠ fkey)
     as Hfkey_notin_nfirst.
     { rewrite Heqn; intros i Hi; lia. }
     clear Heqn.
+    generalize ((if decide (ridx_empty = cnull) then (Z.of_nat 0) else (-1)%Z) ); intros nidx_empty.
 
-    iLöb as "IH" forall (n Hn Hfkey_notin_nfirst).
+    iLöb as "IH" forall (n nidx_empty Hn Hfkey_notin_nfirst).
 
     (* sub rscratch SIZE_MAP ridx; *)
     iDestruct "Hrscratch" as "[%wrscratch Hrscratch]".
@@ -96,8 +104,7 @@ Section KVS_search.
       iDestruct (isKVS_indom_idx with "HKVS") as "%Hidx".
       { by apply elem_of_dom_2 in Hm_idx. }
       exfalso.
-      apply Hfkey_notin_nfirst in Hidx as (k' & w' & Hm_idx' & Hneq_keys).
-      rewrite Hm_idx in Hm_idx'; simplify_eq.
+      eapply Hfkey_notin_nfirst; eauto.
     }
     assert (0 ≤ n < SIZE_MAP)%Z as Hn' by lia.
     (* jnz (".loop_body")%asm rscratch; *)
@@ -106,75 +113,155 @@ Section KVS_search.
 
     destruct (decide (Z.of_nat idx = n)%Z) as [<- | Hneq'].
     - iDestruct (open_isKVS_kvs_frag_idx with "[$HKVS $Hkvs_frag]") as "(HKVS & (Hbk & Hbw & Hfkey) & Hkvs_frag)".
-      replace (cgp_b ^+ 2 * idx)%a  with (cgp_b ^+ (2 * idx))%a by solve_addr+Hn.
       (* load rscratch cgp; *)
       iInstr "Hcode".
       { split; [done |solve_addr]. }
-      (* sub rscratch rkey rscratch; *)
-      iInstr "Hcode".
-      (* jnz (".not_same_key")%asm rscratch; *)
-      replace (fkey - (fkey, w).1)%Z with 0%Z by (cbn;lia).
-      iInstr "Hcode".
-      (* jmp (".loop_end_found")%asm; *)
+      iEval (cbn) in "Hrscratch".
+      (* jnz (".some_index")%asm rscratch; *)
       iInstr "Hcode".
 
-      cbn.
+      (* lea cgp 1; *)
+      iInstr "Hcode".
+      { transitivity (Some ((cgp_b ^+ (3 * idx + 1))%a)); solve_addr. }
+      (* load rscratch cgp; *)
+      iInstr "Hcode".
+      { split; [done |solve_addr]. }
+      iEval (cbn) in "Hrscratch".
+      (* sub rscratch rkey rscratch; *)
+      iInstr "Hcode".
+      replace (fkey - fkey)%Z with 0%Z by (cbn;lia).
+      (* jnz (".not_same_key")%asm rscratch; *)
+      iInstr "Hcode".
+      (* lea cgp (-1)%Z; *)
+      iInstr "Hcode".
+      { transitivity (Some (cgp_b ^+ 3 * idx)%a); solve_addr. }
+      (* jmp (".loop_end_found")%asm; *)
+      iInstr "Hcode".
       iApply "Hpost"; iFrame.
       iPureIntro; rewrite /withinBounds; solve_addr.
 
     - iDestruct (open_isKVS_kvs_frag_idx_diff _ _ _ _ (Z.to_nat n) with "[$HKVS $Hkvs_frag]")
-        as "(%k' & %w' & %Hkk' & %Hm_idx' & HKVS  & Hkvs_frag & (Hbk & Hbw & Hfkey))"
+        as "(%opt_kw' & Hkvs_frag & HKVS & %Hm_idx' & Hkvs_entry & %Hopt_kw')"
       ; auto; try lia.
-      replace (cgp_b ^+ 2 * Z.to_nat n)%a  with (cgp_b ^+ (2 * n))%a by solve_addr+Hn.
-      replace (cgp_b ^+ (2 * Z.to_nat n + 1))%a with (cgp_b ^+ (2 * n + 1))%a by solve_addr+Hn.
+      rewrite /isKVS_entry.
+      iAssert (
+          (cgp_b ^+ 3 * Z.to_nat n)%a ↦ₐ
+            (match opt_kw' with
+             | Some (k,w) => WInt ASM_SOME
+             | None => WInt ASM_NONE
+             end)
+          ∗
+            (cgp_b ^+ (3 * Z.to_nat n + 1))%a ↦ₐ
+              (match opt_kw' with
+               | Some (k,w) => WInt k
+               | None => WInt EMPTY_SLOT
+               end)
+          ∗
+            (cgp_b ^+ (3 * Z.to_nat n + 2))%a ↦ₐ
+              (match opt_kw' with
+               | Some (k,w) => w
+               | None => WInt DEFAULT_VAL
+               end)
+          ∗ (match opt_kw' with | Some _ => True | None => (Z.to_nat n) ⤇(KVS) NONE end)
+        )%I with "[Hkvs_entry]" as "(Hn0 & Hn1 & Hn2 & Hfkey)".
+      { destruct opt_kw' as [ [k' w'] | ]; iFrame.
+        iDestruct "Hkvs_entry" as "($&$&$)"; auto.
+      }
+      replace (cgp_b ^+ 3 * Z.to_nat n)%a  with (cgp_b ^+ (3 * n))%a by solve_addr+Hn.
+      replace (cgp_b ^+ (3 * Z.to_nat n + 1))%a with (cgp_b ^+ (3 * n + 1))%a by solve_addr+Hn.
+      replace (cgp_b ^+ (3 * Z.to_nat n + 2))%a with (cgp_b ^+ (3 * n + 2))%a by solve_addr+Hn.
       (* load rscratch cgp; *)
       iInstr "Hcode".
       { split; [done | solve_addr]. }
-      (* sub rscratch rkey rscratch; *)
-      iInstr "Hcode".
-      (* jnz (".not_same_key")%asm rscratch; *)
-      iInstr "Hcode".
-      { injection; cbn; lia. }
-      (* lea cgp 2; *)
-      iInstr "Hcode".
-      { transitivity (Some ( (cgp_b ^+ (2 * (n+1)))%a)); solve_addr. }
-      (* add ridx ridx 1; *)
-      iInstr "Hcode".
-      (* jmp (".loop_start"); *)
-      iInstr "Hcode".
-      { transitivity (Some ( (pc_a ^+ 1)%a)); solve_addr. }
+      iEval (cbn) in "Hrscratch".
 
-      iDestruct (close_isKVS with "[$HKVS Hbk Hbw Hfkey]") as "HKVS";eauto.
-      {
-        replace (cgp_b ^+ (2 * n))%a with (cgp_b ^+ 2 * Z.to_nat n)%a by solve_addr+Hn.
-        replace (cgp_b ^+ (2 * n + 1))%a  with (cgp_b ^+ (2 * Z.to_nat n + 1))%a by solve_addr+Hn.
-        iFrame.
-      }
+      destruct opt_kw' as [ [k' w'] | ].
+      + (* jnz (".some_index")%asm rscratch; *)
+        iInstr "Hcode".
+        (* lea cgp 1; *)
+        iInstr "Hcode".
+        { transitivity (Some ((cgp_b ^+ (3 * n + 1))%a)); solve_addr+Hn Hn' Hcgp_bound. }
+        (* load rscratch cgp; *)
+        iInstr "Hcode".
+        { split; [done | solve_addr]. }
+        (* sub rscratch rkey rscratch; *)
+        iInstr "Hcode".
+        (* jnz (".not_same_key")%asm rscratch; *)
+        iInstr "Hcode".
+        { injection; cbn; intro; apply Hopt_kw'; cbn; lia. }
+        (* lea cgp 2; *)
+        iInstr "Hcode".
+        { transitivity (Some ( (cgp_b ^+ (3 * (n+1)))%a)); solve_addr+Hn Hn' Hcgp_bound. }
+        (* add ridx ridx 1; *)
+        iInstr "Hcode".
+        (* jmp (".loop_start"); *)
+        iInstr "Hcode".
+        { transitivity (Some ( (pc_a ^+ 2)%a)); solve_addr. }
 
-      iApply ("IH" with "[] [] [$Hcgp] [$Hrkey] [$Hrscratch] [$HKVS] [$Hkvs_frag] [$Hpost] [$Hcode] [$HPC] [$Hridx]").
-      + iPureIntro; lia.
-      + iPureIntro.
-        intros idx' Hidx'_bound.
-        destruct (decide (idx' = Z.to_nat n)%Z) as [-> | Hidx']; eauto.
-        apply Hfkey_notin_nfirst; lia.
+        iDestruct (close_isKVS with "[$HKVS Hn0 Hn1 Hn2]") as "HKVS";eauto.
+        {
+          replace (cgp_b ^+ (3 * n))%a with (cgp_b ^+ 3 * Z.to_nat n)%a by solve_addr+Hn.
+          replace (cgp_b ^+ (3 * n + 1))%a  with (cgp_b ^+ (3 * Z.to_nat n + 1))%a by solve_addr+Hn.
+          replace (cgp_b ^+ (3 * n + 2))%a  with (cgp_b ^+ (3 * Z.to_nat n + 2))%a by solve_addr+Hn.
+          iFrame.
+        }
+
+        iApply ("IH" with
+                 "[] [] [$Hcgp] [$Hrkey] [$Hrscratch] [$HKVS] [$Hkvs_frag] [$Hpost] [$Hridx] [$Hcode] [$HPC] [$Hridx_empty]").
+        * iPureIntro; lia.
+        * iPureIntro.
+          intros idx0 Hidx0_bound k0 w0 Hidx0.
+          destruct (decide (idx0 = Z.to_nat n)%Z) as [-> | Hidx']; eauto.
+          { rewrite Hm_idx' in Hidx0; simplify_map_eq; done. }
+          { eapply Hfkey_notin_nfirst; eauto; lia. }
+      + (* jnz (".some_index")%asm rscratch; *)
+        iInstr "Hcode".
+        (* mov ridx_empty ridx; *)
+        iInstr "Hcode".
+        (* lea cgp 3; *)
+        iInstr "Hcode".
+        { transitivity (Some ((cgp_b ^+ 3 * (n + 1))%a)); solve_addr+Hn Hn' Hcgp_bound. }
+        (* add ridx ridx 1; *)
+        iInstr "Hcode".
+        (* jmp (".loop_start"); *)
+        iInstr "Hcode".
+        { transitivity (Some ( (pc_a ^+ 2)%a)); solve_addr. }
+        iDestruct (close_isKVS with "[$HKVS Hn0 Hn1 Hn2 Hfkey]") as "HKVS";eauto.
+        {
+          replace (cgp_b ^+ (3 * n))%a with (cgp_b ^+ 3 * Z.to_nat n)%a by solve_addr+Hn.
+          replace (cgp_b ^+ (3 * n + 1))%a  with (cgp_b ^+ (3 * Z.to_nat n + 1))%a by solve_addr+Hn.
+          replace (cgp_b ^+ (3 * n + 2))%a  with (cgp_b ^+ (3 * Z.to_nat n + 2))%a by solve_addr+Hn.
+          iFrame.
+        }
+
+        iApply ("IH" with
+                 "[] [] [$Hcgp] [$Hrkey] [$Hrscratch] [$HKVS] [$Hkvs_frag] [$Hpost] [$Hridx] [$Hcode] [$HPC] [$Hridx_empty]").
+        * iPureIntro; lia.
+        * iPureIntro.
+          intros idx0 Hidx0_bound k0 w0 Hidx0.
+          destruct (decide (idx0 = Z.to_nat n)%Z) as [-> | Hidx']; eauto.
+          { rewrite Hm_idx' in Hidx0; simplify_map_eq; done. }
+          { eapply Hfkey_notin_nfirst; eauto; lia. }
   Qed.
 
-  Lemma KVS_search_spec_notin `{KVS : kvsLayout}
+  Lemma KVS_search_spec_empty_slot `{KVS : kvsLayout}
     (pc_b pc_e pc_a : Addr)
     (cgp_b cgp_e : Addr)
-    (rkey ridx rscratch : RegName)
+    (rkey ridx ridx_empty rscratch : RegName)
     (m : kvs_map) (s : kvs_alloc) (s' : gset Z) (ku kn : Z)
     :
-    let instrs := (kvs_search_instrs rkey ridx rscratch) in
+    let instrs := (kvs_search_instrs rkey ridx ridx_empty  rscratch) in
     let fkey := kvs_full_key ku kn in
     SubBounds pc_b pc_e pc_a (pc_a ^+ length instrs)%a ->
     withinBounds cgp_b cgp_e cgp_b = true ->
-    ((cgp_b + (2*SIZE_MAP)%Z)%a = Some cgp_e)%a ->
+    ((cgp_b + (3*SIZE_MAP)%Z)%a = Some cgp_e)%a ->
+
     kn ∉ s' ->
     wf_kvs_full_key ku kn ->
 
     rscratch ≠ cnull ->
     ridx ≠ cnull ->
+    ridx_empty ≠ cnull ->
     rkey ≠ cnull ->
 
     (
@@ -182,150 +269,31 @@ Section KVS_search.
       cgp ↦ᵣ WCap RW Global cgp_b cgp_e cgp_b ∗
       rkey ↦ᵣ WInt fkey ∗
       ridx ↦ᵣ - ∗
+      ridx_empty ↦ᵣ - ∗
       rscratch ↦ᵣ - ∗
 
       isKVS cgp_b m s ∗
       ◯(ALLOC)[ku] s' ∗
 
       codefrag pc_a instrs ∗
-      ▷ (
-          PC ↦ᵣ WCap RX Global pc_b pc_e (pc_a ^+ length instrs)%a ∗
-          cgp ↦ᵣ WCap RW Global cgp_b cgp_e cgp_b ∗
-          rkey ↦ᵣ WInt fkey ∗
-          ridx ↦ᵣ WInt (-1) ∗
-          rscratch ↦ᵣ - ∗
-
-          isKVS cgp_b m s ∗
-          ◯(ALLOC)[ku] s' ∗
-
-          codefrag pc_a instrs -∗
-
-          WP Seq (Instr Executable) {{ v, ⌜v = HaltedV⌝ → na_own cerise_nais ⊤ }}
-        )
-      ⊢ WP Seq (Instr Executable) {{ v, ⌜v = HaltedV⌝ → na_own cerise_nais ⊤ }})%I.
-  Proof.
-    intros instrs fkey ; subst instrs.
-    iIntros (HsubBounds Hbounds_cgp Hcgp_bound Hs' Hwf_full_key Hrscratch Hridx Hkey)
-      "(HPC & Hcgp & Hrkey & [%wridx Hridx] & Hrscratch & HKVS & Halloc & Hcode & Hpost)".
-    codefrag_facts "Hcode"; rename H into Hpc_contiguous ; clear H0.
-
-    (* Mov ridx 0 *)
-    iInstr "Hcode".
-
-    remember 0%Z as n.
-    iAssert (⌜ (0 <= n <= SIZE_MAP)%Z ⌝)%I as "%Hn"; first (iPureIntro ; lia).
-    rewrite{2} (_ : cgp_b = (cgp_b ^+ (2 * n))%a); last by solve_addr.
-    assert (forall i, (0 <= i < Z.to_nat n) -> ∃ (k : Z) (w : Word),  m !! i = Some (k,w) ∧ k ≠ fkey)
-    as Hfkey_notin_nfirst.
-    { rewrite Heqn; intros i Hi; lia. }
-    clear Heqn.
-
-    iLöb as "IH" forall (n Hn Hfkey_notin_nfirst).
-
-    (* sub rscratch SIZE_MAP ridx; *)
-    iDestruct "Hrscratch" as "[%wrscratch Hrscratch]".
-    iInstr "Hcode".
-    replace 16 with SIZE_MAP by (by rewrite /SIZE_MAP).
-    destruct (decide ((SIZE_MAP - n) = 0)%Z) as [Hneq|Hneq].
-    { (* End of the loop. *)
-      rewrite Hneq.
-      assert ( n = SIZE_MAP ) as -> by lia.
-
-      (* jnz (".loop_body")%asm rscratch; *)
-      iInstr "Hcode".
-      (* jmp (".loop_end_not_found")%asm; *)
-      iInstr "Hcode".
-
-      (* lea cgp (-(2*SIZE_MAP))%Z; *)
-      iInstr "Hcode".
-      { transitivity (Some cgp_b); rewrite /SIZE_MAP in Hcgp_bound |- *; solve_addr. }
-      (* mov ridx (-1)%Z; *)
-      iInstr "Hcode".
-      rewrite decide_False //=.
-      iApply "Hpost"; iFrame.
-    }
-    assert (0 ≤ n < SIZE_MAP)%Z as Hn' by lia.
-    (* jnz (".loop_body")%asm rscratch; *)
-    iInstr "Hcode".
-    { by injection. }
-
-  iDestruct (open_isKVS_not_alloc _ _ _ _ (Z.to_nat n) with "HKVS Halloc")
-    as "(%kidx' & %widx & %Hkidx_ne & %Hm_kidx & HKVS & Halloc & (Hbk & Hbw & Hfkey))" ; eauto; [lia|].
-  replace (cgp_b ^+ 2 * Z.to_nat n)%a  with (cgp_b ^+ (2 * n))%a by solve_addr+Hn.
-  replace (cgp_b ^+ (2 * Z.to_nat n + 1))%a with (cgp_b ^+ (1 + 2 * n))%a by solve_addr+Hn.
-
-  (* load rscratch cgp; *)
-  iInstr "Hcode".
-  { split; [done | solve_addr]. }
-  (* sub rscratch rkey rscratch; *)
-  iInstr "Hcode".
-  (* jnz (".not_same_key")%asm rscratch; *)
-  iInstr "Hcode".
-  { injection; cbn; lia. }
-  (* lea cgp 2; *)
-  iInstr "Hcode".
-  { transitivity (Some ( (cgp_b ^+ (2 * (n+1)))%a)); solve_addr. }
-  (* add ridx ridx 1; *)
-  iInstr "Hcode".
-  (* jmp (".loop_start"); *)
-  iInstr "Hcode".
-  { transitivity (Some ( (pc_a ^+ 1)%a)); solve_addr. }
-
-  iDestruct (close_isKVS with "[$HKVS Hbk Hbw Hfkey]") as "HKVS";eauto.
-  {
-    replace (cgp_b ^+ (2 * n))%a with (cgp_b ^+ 2 * Z.to_nat n)%a by solve_addr+Hn.
-    replace (cgp_b ^+ (1 + 2 * n))%a  with (cgp_b ^+ (2 * Z.to_nat n + 1))%a by solve_addr+Hn.
-    iFrame.
-  }
-
-  iApply ("IH" with "[] [] [$Hcgp] [$Hrkey] [$Hrscratch] [$HKVS] [$Halloc] [$Hpost] [$Hcode] [$HPC] [$Hridx]").
-    + iPureIntro; lia.
-    + iPureIntro.
-      intros idx' Hidx'_bound.
-      destruct (decide (idx' = Z.to_nat n)%Z) as [-> | Hidx']; eauto.
-      apply Hfkey_notin_nfirst; lia.
-  Qed.
-
-  Lemma KVS_search_spec_empty_slot `{KVS : kvsLayout}
-    (pc_b pc_e pc_a : Addr)
-    (cgp_b cgp_e : Addr)
-    (rkey ridx rscratch : RegName)
-    (m : kvs_map) (s : kvs_alloc)
-    :
-    let instrs := (kvs_search_instrs rkey ridx rscratch) in
-    SubBounds pc_b pc_e pc_a (pc_a ^+ length instrs)%a ->
-    withinBounds cgp_b cgp_e cgp_b = true ->
-    ((cgp_b + (2*SIZE_MAP)%Z)%a = Some cgp_e)%a ->
-
-    rscratch ≠ cnull ->
-    ridx ≠ cnull ->
-    rkey ≠ cnull ->
-
-    (
-      PC ↦ᵣ WCap RX Global pc_b pc_e pc_a ∗
-      cgp ↦ᵣ WCap RW Global cgp_b cgp_e cgp_b ∗
-      rkey ↦ᵣ WInt EMPTY_SLOT ∗
-      ridx ↦ᵣ - ∗
-      rscratch ↦ᵣ - ∗
-
-      isKVS cgp_b m s ∗
-
-      codefrag pc_a instrs ∗
       ▷ ( (* An empty slot was found*)
           ( ∃ idx_empty_slot : nat,
             (
             PC ↦ᵣ WCap RX Global pc_b pc_e (pc_a ^+ length instrs)%a ∗
-            cgp ↦ᵣ WCap RW Global cgp_b cgp_e (cgp_b ^+ (2*idx_empty_slot))%a ∗
-            rkey ↦ᵣ WInt EMPTY_SLOT ∗
-            ridx ↦ᵣ WInt idx_empty_slot ∗
+            cgp ↦ᵣ WCap RW Global cgp_b cgp_e cgp_b ∗
+            rkey ↦ᵣ WInt fkey ∗
+            ridx ↦ᵣ WInt (-1)%Z ∗
+            ridx_empty ↦ᵣ WInt idx_empty_slot ∗
             rscratch ↦ᵣ - ∗
 
+            ◯(ALLOC)[ku] s' ∗
             isKVS_open cgp_b m s idx_empty_slot ∗
-            (cgp_b ^+ (2*idx_empty_slot))%a ↦ₐ WInt EMPTY_SLOT ∗
-            (cgp_b ^+ (2*idx_empty_slot + 1))%a ↦ₐ WInt DEFAULT_VAL ∗
-            EMPTY_SLOT ⤇(KVS)[ idx_empty_slot ] WInt DEFAULT_VAL ∗
+            (cgp_b ^+ (3*idx_empty_slot))%a ↦ₐ WInt ASM_NONE ∗
+            (cgp_b ^+ (3*idx_empty_slot + 1))%a ↦ₐ WInt EMPTY_SLOT ∗
+            (cgp_b ^+ (3*idx_empty_slot + 2))%a ↦ₐ WInt DEFAULT_VAL ∗
+            idx_empty_slot ⤇(KVS) NONE ∗
 
-            ⌜ withinBounds cgp_b cgp_e (cgp_b ^+ (2 * idx_empty_slot + 1))%a = true ⌝ ∗
+            ⌜ withinBounds cgp_b cgp_e (cgp_b ^+ (3 * idx_empty_slot + 2))%a = true ⌝ ∗
             ⌜ 0 <= idx_empty_slot ⌝ ∗
 
             codefrag pc_a instrs
@@ -335,10 +303,12 @@ Section KVS_search.
             (
               PC ↦ᵣ WCap RX Global pc_b pc_e (pc_a ^+ length instrs)%a ∗
               cgp ↦ᵣ WCap RW Global cgp_b cgp_e cgp_b ∗
-              rkey ↦ᵣ WInt EMPTY_SLOT ∗
+              rkey ↦ᵣ WInt fkey ∗
               ridx ↦ᵣ WInt (-1) ∗
+              ridx_empty ↦ᵣ WInt (-1) ∗
               rscratch ↦ᵣ - ∗
 
+              ◯(ALLOC)[ku] s' ∗
               isKVS cgp_b m s ∗
 
               codefrag pc_a instrs
@@ -347,21 +317,49 @@ Section KVS_search.
         )
       ⊢ WP Seq (Instr Executable) {{ v, ⌜v = HaltedV⌝ → na_own cerise_nais ⊤ }})%I.
   Proof.
-    intros instrs ; subst instrs.
-    iIntros (HsubBounds Hbounds_cgp Hcgp_bound Hrscratch Hridx Hkey)
-      "(HPC & Hcgp & Hrkey & [%wridx Hridx] & Hrscratch & HKVS & Hcode & Hpost)".
+    intros instrs fkey ; subst instrs.
+    iIntros (HsubBounds Hbounds_cgp Hcgp_bound Hs' Hwf_full_key Hrscratch Hridx Hridx_empty Hkey)
+      "(HPC & Hcgp & Hrkey & [%wridx Hridx] & [%wridx_empty Hridx_empty] & Hrscratch & HKVS & Halloc & Hcode & Hpost)".
     codefrag_facts "Hcode"; rename H into Hpc_contiguous ; clear H0.
 
-    (* Mov ridx 0 *)
+    (* mov ridx 0%Z; *)
     iInstr "Hcode".
+    (* mov ridx_empty (-1)%Z; *)
+    iInstr "Hcode".
+    destruct (decide (ridx_empty = cnull)) as [|_]; first done.
+    remember (-1)%Z as idx_empty.
+    rewrite {1}Heqidx_empty.
+    rewrite {1}Heqidx_empty.
+    rewrite {1}Heqidx_empty.
 
     remember 0%Z as n.
     iAssert (⌜ (0 <= n <= SIZE_MAP)%Z ⌝)%I as "%Hn"; first (iPureIntro ; lia).
-    rewrite{2} (_ : cgp_b = (cgp_b ^+ (2 * n))%a); last by solve_addr.
-    assert (forall i, (0 <= i < Z.to_nat n) -> ∃ (k : Z) (w : Word),  m !! i = Some (k,w) ∧ k ≠ EMPTY_SLOT)
+    rewrite{2} (_ : cgp_b = (cgp_b ^+ (3 * n))%a); last by solve_addr.
+    assert (forall i, (0 <= i < Z.to_nat n) -> ∀ (k : Z) (w : Word), m !! i = Some (Some (k,w)) -> k ≠ fkey)
     as Hfkey_notin_nfirst.
     { rewrite Heqn; intros i Hi; lia. }
-    clear Heqn.
+
+    iAssert (
+       if (decide ((Forall (fun idx => m !! idx ≠ Some None) (seq 0 (Z.to_nat n)))))
+       then (isKVS cgp_b m s ∗
+             ridx_empty ↦ᵣ WInt (-1)
+            )
+       else ( ∃ (idx_empty : nat),
+                ⌜ 0 <= idx_empty < (Z.to_nat n)⌝ ∗
+                isKVS_open cgp_b m s idx_empty ∗
+                (cgp_b ^+ 3 * idx_empty)%a ↦ₐ WInt ASM_NONE ∗
+                (cgp_b ^+ (3 * idx_empty + 1))%a ↦ₐ WInt EMPTY_SLOT ∗
+                (cgp_b ^+ (3 * idx_empty + 2))%a ↦ₐ WInt DEFAULT_VAL ∗
+                pointsto idx_empty (DfracOwn 1) None ∗
+                ridx_empty ↦ᵣ WInt idx_empty
+            )
+      )%I with "[HKVS Hridx_empty]" as "Hloop_inv".
+    {
+      destruct ( decide (Forall (λ idx : nat, m !! idx ≠ Some None) (seq 0 (Z.to_nat n))) ) as [|Hcontra]; rewrite Heqidx_empty; iFrame.
+      exfalso; apply Hcontra.
+      rewrite Heqn /=; apply Forall_nil; done.
+    }
+    clear Heqn Heqidx_empty.
 
     iLöb as "IH" forall (n Hn Hfkey_notin_nfirst).
 
@@ -378,79 +376,307 @@ Section KVS_search.
       iInstr "Hcode".
       (* jmp (".loop_end_not_found")%asm; *)
       iInstr "Hcode".
-
-      (* lea cgp (-(2*SIZE_MAP))%Z; *)
+      (* lea cgp (-(3*SIZE_MAP))%Z; *)
       iInstr "Hcode".
       { transitivity (Some cgp_b); rewrite /SIZE_MAP in Hcgp_bound |- *; solve_addr. }
       (* mov ridx (-1)%Z; *)
       iInstr "Hcode".
-      rewrite decide_False //=.
-      iApply "Hpost"; iRight; iFrame.
+      rewrite (decide_False (Z.of_nat 0)); last done.
+
+      destruct ( decide ( (Forall (λ idx : nat, m !! idx ≠ Some None) (seq 0 (Z.to_nat SIZE_MAP))) )) as [Hnone|Hnone].
+      - iDestruct "Hloop_inv" as "(HKVS & Hridx_empty)".
+        iApply "Hpost"; iRight; iFrame.
+
+      - iDestruct "Hloop_inv" as
+          "(%idx_empty_found & %Hidx_empty_found & HKVS & Hn0 & Hn1 & Hn2 & Hfkey & Hridx_empty)".
+        iApply "Hpost"; iLeft; iFrame.
+        iPureIntro; split; solve_addr.
     }
     assert (0 ≤ n < SIZE_MAP)%Z as Hn' by lia.
     (* jnz (".loop_body")%asm rscratch; *)
     iInstr "Hcode".
     { by injection. }
 
-  iDestruct (open_isKVS _ _ _ (Z.to_nat n) with "HKVS") as "(%kidx' & %widx & %Hm_kidx & HKVS & (Hbk & Hbw & Hfkey))"
-  ; eauto; [lia|].
-  replace (cgp_b ^+ 2 * Z.to_nat n)%a  with (cgp_b ^+ (2 * n))%a by solve_addr+Hn.
-  replace (cgp_b ^+ (2 * Z.to_nat n + 1))%a with (cgp_b ^+ (2 * n + 1))%a by solve_addr+Hn.
-  iEval (cbn) in "Hbk"; iEval (cbn) in "Hbw"; iEval (cbn) in "Hfkey".
+    destruct ( decide (Forall (λ idx : nat, m !! idx ≠ Some None) (seq 0 (Z.to_nat n))) ) as [Hnone | Hnone].
+    - (* No empty slot have been found yet *)
+      iDestruct "Hloop_inv" as "(HKVS & Hridx_empty)".
 
-  (* load rscratch cgp; *)
-  iInstr "Hcode".
-  { split; [done | solve_addr]. }
-  (* sub rscratch rkey rscratch; *)
-  iInstr "Hcode".
+      iDestruct (open_isKVS_not_alloc _ _ _ _ (Z.to_nat n) with "HKVS Halloc")
+        as "(%opt_kwidx & %Hm_kwidx & HKVS & Halloc & Hfkey & %Hneq_fkey)" ; eauto; [lia|].
 
-  rewrite /isKVS_entry_empty.
-  destruct (decide (kidx' = EMPTY_SLOT)) as [Hkidx'_empty |  Hkidx'_empty]; simplify_eq.
-  - (* Empty slot found *)
-    replace (Z.sub EMPTY_SLOT EMPTY_SLOT) with 0%Z by lia.
-    (* jnz (".not_same_key")%asm rscratch; *)
-    iInstr "Hcode".
-    (* jmp (".loop_end_found")%asm; *)
-    iInstr "Hcode".
+      iAssert (
+          (cgp_b ^+ 3 * Z.to_nat n)%a ↦ₐ
+            (match opt_kwidx with
+             | Some (k,w) => WInt ASM_SOME
+             | None => WInt ASM_NONE
+             end)
+          ∗
+            (cgp_b ^+ (3 * Z.to_nat n + 1))%a ↦ₐ
+              (match opt_kwidx with
+               | Some (k,w) => WInt k
+               | None => WInt EMPTY_SLOT
+               end)
+          ∗
+            (cgp_b ^+ (3 * Z.to_nat n + 2))%a ↦ₐ
+              (match opt_kwidx with
+               | Some (k,w) => w
+               | None => WInt DEFAULT_VAL
+               end)
+          ∗ (match opt_kwidx with | Some _ => True | None => (Z.to_nat n) ⤇(KVS) NONE end)
+        )%I with "[Hfkey]" as "(Hn0 & Hn1 & Hn2 & Hfkey)".
+      { destruct opt_kwidx as [ [kidx widx] | ]; iFrame.
+        iDestruct "Hfkey" as "($&$&$)"; auto.
+      }
+      replace (cgp_b ^+ 3 * Z.to_nat n)%a  with (cgp_b ^+ (3 * n))%a by solve_addr+Hn.
+      replace (cgp_b ^+ (3 * Z.to_nat n + 1))%a with (cgp_b ^+ (3 * n + 1))%a by solve_addr+Hn.
+      replace (cgp_b ^+ (3 * Z.to_nat n + 2))%a with (cgp_b ^+ (3 * n + 2))%a by solve_addr+Hn.
 
-    iDestruct (isKVS_open_valid with "HKVS Hfkey") as "%Hm_kidx_eq"; simplify_map_eq.
-    replace (cgp_b ^+ (2 * n))%a with (cgp_b ^+ (2 * Z.to_nat n))%a by solve_addr+Hn.
-    replace (cgp_b ^+ (2 * n + 1))%a  with (cgp_b ^+ (2 * Z.to_nat n + 1))%a by solve_addr+Hn.
+      (* load rscratch cgp; *)
+      iInstr "Hcode".
+      { split; [done |solve_addr]. }
+      iEval (cbn) in "Hrscratch".
+
+      destruct opt_kwidx as [ [kidx widx] | ].
+      + (* This is not an empty slot. Because we know that fkey ∉ s, the key will not match *)
+        (* jnz (".some_index")%asm rscratch; *)
+        iInstr "Hcode".
+
+        (* lea cgp 1; *)
+        iInstr "Hcode".
+        { transitivity (Some ((cgp_b ^+ (3 * n + 1))%a)); solve_addr+Hn Hn' Hcgp_bound. }
+        (* load rscratch cgp; *)
+        iInstr "Hcode".
+        { split; [done |solve_addr]. }
+        (* sub rscratch rkey rscratch; *)
+        iInstr "Hcode".
+        assert ( WInt (fkey - kidx)%Z ≠ WInt 0 ) as Hfkey_neq.
+        { injection; intro; simplify_eq; apply Hneq_fkey; cbn; lia. }
+        (* jnz (".not_same_key")%asm rscratch; *)
+        iInstr "Hcode".
+
+        (* lea cgp 2; *)
+        iInstr "Hcode".
+        { transitivity (Some ((cgp_b ^+ (3 * n + 3))%a)); solve_addr+Hn Hn' Hcgp_bound. }
+        (* add ridx ridx 1; *)
+        iInstr "Hcode".
+        (* jmp (".loop_start"); *)
+        iInstr "Hcode".
+        { transitivity (Some ( (pc_a ^+ 2)%a)); solve_addr. }
+
+        iDestruct (close_isKVS with "[$HKVS Hn0 Hn1 Hn2 Hfkey]") as "HKVS";eauto.
+        {
+          replace (cgp_b ^+ (3 * n))%a with (cgp_b ^+ 3 * Z.to_nat n)%a by solve_addr+Hn.
+          replace (cgp_b ^+ (3 * n + 1))%a  with (cgp_b ^+ (3 * Z.to_nat n + 1))%a by solve_addr+Hn.
+          replace (cgp_b ^+ (3 * n + 2))%a  with (cgp_b ^+ (3 * Z.to_nat n + 2))%a by solve_addr+Hn.
+          iFrame.
+        }
+        replace (cgp_b ^+ (3 * n + 3))%a with (cgp_b ^+ (3 * (n + 1)))%a by solve_addr+ Hn Hn' Hcgp_bound.
+
+        iApply ("IH" with "[] [] [$Hcgp] [$Hrkey] [$Hrscratch] [$Halloc]
+         [$Hpost] [$Hridx] [$Hcode] [$HPC] [HKVS Hridx_empty]").
+        * iPureIntro; lia.
+        * iPureIntro.
+          intros idx0 Hidx0_bound k0 w0 Hidx0.
+          destruct (decide (idx0 = Z.to_nat n)%Z) as [-> | Hidx']; eauto.
+          { rewrite Hm_kwidx in Hidx0; simplify_map_eq; done. }
+          { eapply Hfkey_notin_nfirst; eauto; lia. }
+        * case_decide as Hnone'; iFrame.
+          exfalso.
+          apply Hnone'.
+          replace ( (seq 0 (Z.to_nat (n + 1))) ) with ( (seq 0 (Z.to_nat n)) ++ [Z.to_nat n] ).
+          2: {
+            replace [Z.to_nat n] with (seq (Z.to_nat n) 1) by done.
+            rewrite -seq_app.
+            replace (Z.to_nat n + 1) with (Z.to_nat (n + 1)) by lia.
+            done.
+          }
+          apply Forall_app; split; auto.
+          apply Forall_singleton.
+          rewrite Hm_kwidx; done.
+      + (* This is an empty slot. We will update ridx_empty and keep KVS open *)
+
+        (* jnz (".some_index")%asm rscratch; *)
+        iInstr "Hcode".
+        (* mov ridx_empty ridx; *)
+        iInstr "Hcode".
+        (* lea cgp 3; *)
+        iInstr "Hcode".
+        { transitivity (Some ((cgp_b ^+ (3 * (n + 1)))%a)); solve_addr+Hn Hn' Hcgp_bound. }
+        (* add ridx ridx 1; *)
+        iInstr "Hcode".
+        (* jmp (".loop_start"); *)
+        iInstr "Hcode".
+        { transitivity (Some ( (pc_a ^+ 2)%a)); solve_addr. }
+
+        rewrite {6}(_ : n = (Z.of_nat (Z.to_nat n))); last lia.
+        replace (cgp_b ^+ (3 * n))%a with (cgp_b ^+ 3 * Z.to_nat n)%a by solve_addr+Hn.
+        replace (cgp_b ^+ (3 * n + 1))%a  with (cgp_b ^+ (3 * Z.to_nat n + 1))%a by solve_addr+Hn.
+        replace (cgp_b ^+ (3 * n + 2))%a  with (cgp_b ^+ (3 * Z.to_nat n + 2))%a by solve_addr+Hn.
+        iApply ("IH" with "[] [] [$Hcgp] [$Hrkey] [$Hrscratch] [$Halloc]
+         [$Hpost] [$Hridx] [$Hcode] [$HPC] [HKVS Hridx_empty Hn0 Hn1 Hn2 Hfkey]").
+        * iPureIntro; lia.
+        * iPureIntro.
+          intros idx0 Hidx0_bound k0 w0 Hidx0.
+          destruct (decide (idx0 = Z.to_nat n)%Z) as [-> | Hidx']; eauto.
+          { rewrite Hm_kwidx in Hidx0; simplify_map_eq; done. }
+          { eapply Hfkey_notin_nfirst; eauto; lia. }
+        * case_decide as Hnone'; iFrame; last (iPureIntro; lia).
+          exfalso.
+          replace ( (seq 0 (Z.to_nat (n + 1))) ) with ( (seq 0 (Z.to_nat n)) ++ [Z.to_nat n] ) in Hnone'.
+          2: {
+            replace [Z.to_nat n] with (seq (Z.to_nat n) 1) by done.
+            rewrite -seq_app.
+            replace (Z.to_nat n + 1) with (Z.to_nat (n + 1)) by lia.
+            done.
+          }
+          apply Forall_app in Hnone' as [_ Hnone'].
+          apply (Forall_singleton _ (Z.to_nat n)) in Hnone'; cbn in *.
+          done.
+
+    - (* An empty slot have already been found *)
+      iDestruct "Hloop_inv" as
+        "(%idx_empty_found & %Hidx_empty_found & HKVS & Hn0 & Hn1 & Hn2 & Hfkey & Hridx_empty)".
+
+      iDestruct (isKVS_open_valid_None with "HKVS Hfkey") as "%Hidx_empty_found'".
+
+      iDestruct (close_isKVS with "[$HKVS Hn0 Hn1 Hn2 Hfkey]") as "HKVS";eauto.
+      { iFrame. }
 
 
-    assert (((Z.of_nat (Z.to_nat n))) = n) as Hn_eq by lia.
-    rewrite -{1}Hn_eq.
-    iApply "Hpost"; iLeft; iFrame.
-    iPureIntro; rewrite /withinBounds; solve_addr.
+      iDestruct (open_isKVS_not_alloc _ _ _ _ (Z.to_nat n) with "HKVS Halloc")
+        as "(%opt_kwidx & %Hm_kwidx & HKVS & Halloc & Hfkey & %Hneq_fkey)" ; eauto; [lia|].
 
-  - (* Empty slot not found *)
+      iAssert (
+          (cgp_b ^+ 3 * Z.to_nat n)%a ↦ₐ
+            (match opt_kwidx with
+             | Some (k,w) => WInt ASM_SOME
+             | None => WInt ASM_NONE
+             end)
+          ∗
+            (cgp_b ^+ (3 * Z.to_nat n + 1))%a ↦ₐ
+              (match opt_kwidx with
+               | Some (k,w) => WInt k
+               | None => WInt EMPTY_SLOT
+               end)
+          ∗
+            (cgp_b ^+ (3 * Z.to_nat n + 2))%a ↦ₐ
+              (match opt_kwidx with
+               | Some (k,w) => w
+               | None => WInt DEFAULT_VAL
+               end)
+          ∗ (match opt_kwidx with | Some _ => True | None => (Z.to_nat n) ⤇(KVS) NONE end)
+        )%I with "[Hfkey]" as "(Hn0 & Hn1 & Hn2 & Hfkey)".
+      { destruct opt_kwidx as [ [kidx widx] | ]; iFrame.
+        iDestruct "Hfkey" as "($&$&$)"; auto.
+      }
+      replace (cgp_b ^+ 3 * Z.to_nat n)%a  with (cgp_b ^+ (3 * n))%a by solve_addr+Hn.
+      replace (cgp_b ^+ (3 * Z.to_nat n + 1))%a with (cgp_b ^+ (3 * n + 1))%a by solve_addr+Hn.
+      replace (cgp_b ^+ (3 * Z.to_nat n + 2))%a with (cgp_b ^+ (3 * n + 2))%a by solve_addr+Hn.
 
-    (* jnz (".not_same_key")%asm rscratch; *)
-    iInstr "Hcode".
-    { injection; cbn; lia. }
-    (* lea cgp 2; *)
-    iInstr "Hcode".
-    { transitivity (Some ( (cgp_b ^+ (2 * (n+1)))%a)); solve_addr. }
-    (* add ridx ridx 1; *)
-    iInstr "Hcode".
-    (* jmp (".loop_start"); *)
-    iInstr "Hcode".
-    { transitivity (Some ( (pc_a ^+ 1)%a)); solve_addr. }
+      (* load rscratch cgp; *)
+      iInstr "Hcode".
+      { split; [done |solve_addr]. }
+      iEval (cbn) in "Hrscratch".
 
-    iDestruct (close_isKVS with "[$HKVS Hbk Hbw Hfkey]") as "HKVS";eauto.
-    {
-      replace (cgp_b ^+ (2 * n))%a with (cgp_b ^+ 2 * Z.to_nat n)%a by solve_addr+Hn.
-      replace (cgp_b ^+ (2 * n + 1))%a  with (cgp_b ^+ (2 * Z.to_nat n + 1))%a by solve_addr+Hn.
-      rewrite /isKVS_entry /isKVS_entry_empty /= decide_False //.
-      iFrame.
-    }
 
-    iApply ("IH" with "[] [] [$Hcgp] [$Hrkey] [$Hrscratch] [$HKVS] [$Hpost] [$Hcode] [$HPC] [$Hridx]").
-    + iPureIntro; lia.
-    + iPureIntro.
-      intros idx' Hidx'_bound.
-      destruct (decide (idx' = Z.to_nat n)%Z) as [-> | Hidx']; eauto.
-      apply Hfkey_notin_nfirst; lia.
+      destruct opt_kwidx as [ [kidx widx] | ].
+      + (* This is not an empty slot. Because we know that fkey ∉ s, the key will not match *)
+        (* jnz (".some_index")%asm rscratch; *)
+        iInstr "Hcode".
+
+        (* lea cgp 1; *)
+        iInstr "Hcode".
+        { transitivity (Some ((cgp_b ^+ (3 * n + 1))%a)); solve_addr+Hn Hn' Hcgp_bound. }
+        (* load rscratch cgp; *)
+        iInstr "Hcode".
+        { split; [done |solve_addr]. }
+        (* sub rscratch rkey rscratch; *)
+        iInstr "Hcode".
+        assert ( WInt (fkey - kidx)%Z ≠ WInt 0 ) as Hfkey_neq.
+        { injection; intro; simplify_eq; apply Hneq_fkey; cbn; lia. }
+        (* jnz (".not_same_key")%asm rscratch; *)
+        iInstr "Hcode".
+
+        (* lea cgp 2; *)
+        iInstr "Hcode".
+        { transitivity (Some ((cgp_b ^+ (3 * n + 3))%a)); solve_addr+Hn Hn' Hcgp_bound. }
+        (* add ridx ridx 1; *)
+        iInstr "Hcode".
+        (* jmp (".loop_start"); *)
+        iInstr "Hcode".
+        { transitivity (Some ( (pc_a ^+ 2)%a)); solve_addr. }
+
+        iDestruct (close_isKVS with "[$HKVS Hn0 Hn1 Hn2 Hfkey]") as "HKVS";eauto.
+        {
+          replace (cgp_b ^+ (3 * n))%a with (cgp_b ^+ 3 * Z.to_nat n)%a by solve_addr+Hn.
+          replace (cgp_b ^+ (3 * n + 1))%a  with (cgp_b ^+ (3 * Z.to_nat n + 1))%a by solve_addr+Hn.
+          replace (cgp_b ^+ (3 * n + 2))%a  with (cgp_b ^+ (3 * Z.to_nat n + 2))%a by solve_addr+Hn.
+          iFrame.
+        }
+        replace (cgp_b ^+ (3 * n + 3))%a with (cgp_b ^+ (3 * (n + 1)))%a by solve_addr + Hn Hn' Hcgp_bound.
+
+        iDestruct (open_isKVS_not_alloc _ _ _ _ idx_empty_found with "HKVS Halloc")
+          as "(%opt_kwidx_empty & %Hm_kwidx_empty & HKVS & Halloc & Hfkey & %Hneq_fkey_empty)" ; eauto; [lia|].
+        rewrite Hidx_empty_found' in Hm_kwidx_empty; simplify_eq.
+        iDestruct "Hfkey" as "(Hn0 & Hn1 & Hn2 & Hfkey)".
+
+        iApply ("IH" with "[] [] [$Hcgp] [$Hrkey] [$Hrscratch] [$Halloc]
+         [$Hpost] [$Hridx] [$Hcode] [$HPC] [HKVS Hn0 Hn1 Hn2 Hfkey Hridx_empty]").
+        * iPureIntro; lia.
+        * iPureIntro.
+          intros idx0 Hidx0_bound k0 w0 Hidx0.
+          clear Hidx_empty_found.
+          destruct (decide (idx0 = Z.to_nat n)%Z) as [-> | Hidx']; eauto.
+          { rewrite Hm_kwidx in Hidx0; simplify_map_eq; done. }
+          { eapply Hfkey_notin_nfirst; eauto; lia. }
+        * case_decide as Hnone'; iFrame; last (iPureIntro; lia).
+          exfalso.
+          rewrite Forall_forall in Hnone'.
+          specialize (Hnone' idx_empty_found).
+          apply Hnone'; auto.
+          apply elem_of_seq; lia.
+
+
+      + (* This is an empty slot. We will update ridx_empty and keep KVS open *)
+
+        (* jnz (".some_index")%asm rscratch; *)
+        iInstr "Hcode".
+        (* mov ridx_empty ridx; *)
+        iInstr "Hcode".
+        (* lea cgp 3; *)
+        iInstr "Hcode".
+        { transitivity (Some ((cgp_b ^+ (3 * (n + 1)))%a)); solve_addr+Hn Hn' Hcgp_bound. }
+        (* add ridx ridx 1; *)
+        iInstr "Hcode".
+        (* jmp (".loop_start"); *)
+        iInstr "Hcode".
+        { transitivity (Some ( (pc_a ^+ 2)%a)); solve_addr. }
+
+        rewrite {6}(_ : n = (Z.of_nat (Z.to_nat n))); last lia.
+        replace (cgp_b ^+ (3 * n))%a with (cgp_b ^+ 3 * Z.to_nat n)%a by solve_addr+Hn.
+        replace (cgp_b ^+ (3 * n + 1))%a  with (cgp_b ^+ (3 * Z.to_nat n + 1))%a by solve_addr+Hn.
+        replace (cgp_b ^+ (3 * n + 2))%a  with (cgp_b ^+ (3 * Z.to_nat n + 2))%a by solve_addr+Hn.
+        iApply ("IH" with "[] [] [$Hcgp] [$Hrkey] [$Hrscratch] [$Halloc]
+         [$Hpost] [$Hridx] [$Hcode] [$HPC] [HKVS Hridx_empty Hn0 Hn1 Hn2 Hfkey]").
+        * iPureIntro; lia.
+        * iPureIntro.
+          intros idx0 Hidx0_bound k0 w0 Hidx0.
+          clear Hidx_empty_found.
+          destruct (decide (idx0 = Z.to_nat n)%Z) as [-> | Hidx']; eauto.
+          { rewrite Hm_kwidx in Hidx0; simplify_map_eq; done. }
+          { eapply Hfkey_notin_nfirst; eauto; lia. }
+        * case_decide as Hnone'; iFrame; last (iPureIntro; lia).
+          exfalso.
+          replace ( (seq 0 (Z.to_nat (n + 1))) ) with ( (seq 0 (Z.to_nat n)) ++ [Z.to_nat n] ) in Hnone'.
+          2: {
+            replace [Z.to_nat n] with (seq (Z.to_nat n) 1) by done.
+            rewrite -seq_app.
+            replace (Z.to_nat n + 1) with (Z.to_nat (n + 1)) by lia.
+            done.
+          }
+          apply Forall_app in Hnone' as [_ Hnone'].
+          apply (Forall_singleton _ (Z.to_nat n)) in Hnone'; cbn in *.
+          done.
   Qed.
 
 End KVS_search.
